Mathlib refactor

Datalog/Spec.lean
@@ -1,10 +1,154 @@
-import Datalog.DSL
+import Mathlib.Tactic
+
 import Datalog.Utils
+
+-- Aliases
+
+abbrev Constant :=
+  String
+
+abbrev Variable :=
+  String
+
+abbrev Relation :=
+  String
+
+abbrev Arity :=
+  Nat
+
+abbrev Predicate :=
+  Relation × Arity
+
+-- Term
+
+inductive Term where
+  | const : Constant → Term
+  | var : Variable → Term
+  deriving DecidableEq
+
+instance : ToString Term where
+  toString
+    | .const c => c
+    | .var v => v
+
+instance : Repr Term where
+  reprPrec term _ := f!"{toString term}"
+
+def Term.isConst : Term → Bool
+  | .const _ => true
+  | _ => false
+
+def Term.isVar : Term → Bool
+  | .var _ => true
+  | _ => false
+
+def Term.constant? : Term → Option Constant
+  | .const c => some c
+  | _ => none
+
+def Term.variable? : Term → Option Variable
+  | .var v => some v
+  | _ => none
+
+-- Atom
+
+structure Atom where
+  rel : Relation
+  terms : List Term
+  deriving DecidableEq
+
+instance : ToString Atom where
+  toString
+    | Atom.mk rel [] => rel
+    | Atom.mk rel terms => rel ++ "(" ++ ", ".intercalate (toString <$> terms) ++ ")"
+
+instance : Repr Atom where
+  reprPrec atom _ := f!"{toString atom}"
+
+def Atom.predicate (atom : Atom) : Predicate :=
+  (atom.rel, atom.terms.length)
+
+def Atom.isGround (atom : Atom) : Bool :=
+  ∀ t ∈ atom.terms, t.isConst
+
+-- Rule
+
+structure Rule where
+  head : Atom
+  body : List Atom
+  deriving DecidableEq
+
+instance : ToString Rule where
+  toString
+    | Rule.mk head [] => toString head ++ "."
+    | Rule.mk head body =>
+      toString head ++ " :- " ++ ", ".intercalate (toString <$> body)
+
+instance : Repr Rule where
+  reprPrec rule _ := f!"{toString rule}"
+
+def Rule.isGround (rule : Rule) : Bool :=
+  rule.head.isGround ∧ ∀ a ∈ rule.body, a.isGround
+
+def Rule.isFact (rule : Rule) : Bool :=
+  rule.body = ∅
+
+-- Program
+
+abbrev Program :=
+  List Rule
+
+instance : ToString Program where
+  toString prog :=
+    "\n".intercalate (toString <$> prog)
+
+instance : Repr Program where
+  reprPrec prog _ := f!"{toString prog}"
+
+-- DSL
+
+declare_syntax_cat datalog_term
+declare_syntax_cat datalog_atom
+declare_syntax_cat datalog_rule
+declare_syntax_cat datalog_prog
+
+syntax ident : datalog_term
+syntax ident ("(" datalog_term,* ")")? : datalog_atom
+syntax datalog_atom (":-" datalog_atom,*)? "." : datalog_rule
+syntax datalog_rule* : datalog_prog
+
+syntax "[Term|" datalog_term "]" : term
+syntax "[Atom|" datalog_atom "]" : term
+syntax "[Rule|" datalog_rule "]" : term
+syntax "[Prog|" datalog_prog "]" : term
+
+open Lean.Syntax (mkStrLit) in
+macro_rules
+  | `([Term| $s:ident]) =>
+    let s := s.getId.toString
+    if s.front.isUpper then `(Term.var $(mkStrLit s)) else `(Term.const $(mkStrLit s))
+  | `([Atom| $rel:ident]) =>
+    `(Atom.mk $(mkStrLit rel.getId.toString) [])
+  | `([Atom| $rel:ident ( $[$terms:datalog_term],* )]) =>
+    `(Atom.mk $(mkStrLit rel.getId.toString) [ $[[Term| $terms]],* ])
+  | `([Rule| $head:datalog_atom .]) =>
+    `(Rule.mk [Atom| $head] [])
+  | `([Rule| $head:datalog_atom :- $[$body:datalog_atom],* .]) =>
+    `(Rule.mk [Atom| $head] [ $[[Atom| $body]],* ])
+  | `([Prog| $[$prog:datalog_rule]*]) =>
+    `(([ $[[Rule| $prog]],* ] : Program))
+
+#check [Prog|
+parent(xerces, brooke).
+parent(brooke, damocles).
+ancestor(X, Y) :- parent(X, Y).
+ancestor(X, Y) :- parent(X, Z), ancestor(Z, Y).
+]
 
 -- Substitution
 
 abbrev Substitution :=
-  String → String
+  Variable → Constant
 
 def Term.applySub (σ : Substitution) : Term → Term
   | .const c => .const c
@@ -13,46 +157,100 @@ def Term.applySub (σ : Substitution) : Term → Term
 def Atom.applySub (σ : Substitution) (atom : Atom) : Atom :=
   Atom.mk atom.rel (atom.terms.map (Term.applySub σ))
 
-theorem isConst_of_mem_applySub {term : Term} {atom : Atom} {σ : Substitution} (h : term ∈ (atom.applySub σ).terms) :
-    term.isConst := by
-  simp [Atom.applySub, Term.applySub] at h
-  simp [Term.isConst]
-  grind
+theorem Term.isConst_of_applySub {σ : Substitution} {term : Term} :
+    term.applySub σ |>.isConst := by
+  simp [Term.isConst, Term.applySub]
+  cases term with simp
+
+theorem Atom.isGround_of_applySub {σ : Substitution} {atom : Atom} :
+    atom.applySub σ |>.isGround := by
+  simp [Atom.isGround, Atom.applySub, Term.isConst_of_applySub]
 
 -- Predicates
 
-def Program.Predicates (prog : Program) (pred : String × Nat) : Prop :=
-  ∃ r ∈ prog, pred = r.head.predicate ∨ ∃ a ∈ r.body, pred = a.predicate
+def Rule.predicates (rule : Rule) :=
+  {rule.head.predicate} ∪ rule.body.toFinset.image Atom.predicate
 
-theorem Program.mem_getPredicates_iff (prog : Program) (pred : String × Nat) :
-    pred ∈ prog.getPredicates ↔ prog.Predicates pred := by
-  simp [Program.getPredicates, Rule.getPredicates, Atom.predicate, Program.Predicates]
+def Program.predicates (prog : Program) : Finset Predicate :=
+  prog.toFinset.biUnion Rule.predicates
+
+#eval Program.predicates [Prog|
+parent(xerces, brooke).
+parent(brooke, damocles).
+ancestor(X, Y) :- parent(X, Y).
+ancestor(X, Y) :- parent(X, Z), ancestor(Z, Y).
+]
+
+theorem Program.mem_predicates {prog : Program} :
+    ∀ p, p ∈ prog.predicates ↔ ∃ r ∈ prog, p = r.head.predicate ∨ ∃ a ∈ r.body, p = a.predicate := by
+  simp [Program.predicates, Rule.predicates]
   grind
 
 -- Constants
 
-def Program.Constants (prog : Program) (t : Term) : Prop :=
-  t.isConst ∧ ∃ r ∈ prog, t ∈ r.head.terms ∨ ∃ a ∈ r.body, t ∈ a.terms
+def Atom.constants (atom : Atom) : Finset Term :=
+  atom.terms.filter Term.isConst |>.toFinset
 
-theorem Program.mem_getConstants_iff (prog : Program) (term : Term) :
-    term ∈ prog.getConstants ↔ prog.Constants term := by
-  simp [Program.getConstants, Rule.getConstants, Atom.getConstants, Program.Constants]
+def Rule.constants (rule : Rule) : Finset Term :=
+  rule.head.constants ∪ rule.body.toFinset.biUnion Atom.constants
+
+def Program.constants (prog : Program) : Finset Term :=
+  prog.toFinset.biUnion Rule.constants
+
+#eval Program.constants [Prog|
+parent(xerces, brooke).
+parent(brooke, damocles).
+ancestor(X, Y) :- parent(X, Y).
+ancestor(X, Y) :- parent(X, Z), ancestor(Z, Y).
+]
+
+theorem Program.mem_constants {prog : Program} :
+    ∀ t, t ∈ prog.constants ↔ t.isConst ∧ ∃ r ∈ prog, t ∈ r.head.terms ∨ ∃ a ∈ r.body, t ∈ a.terms := by
+  simp [Program.constants, Rule.constants, Atom.constants]
   grind
 
 -- Herbrand base
 
-def Program.HerbrandBase (prog : Program) (a : Atom) : Prop :=
-  prog.Predicates a.predicate ∧ ∀ t ∈ a.terms, prog.Constants t
+def Program.hb (prog : Program) : Finset Atom :=
+  prog.predicates.biUnion (fun (rel, arity) =>
+    prog.constants.cartesianPower arity |>.image (fun terms =>
+      Atom.mk rel terms))
 
-theorem Program.mem_getHerbrandBase_iff (prog : Program) (atom : Atom) :
-    atom ∈ prog.getHerbrandBase ↔ prog.HerbrandBase atom := by
-  simp [Program.getHerbrandBase, Program.mem_getPredicates_iff, List.mem_product_iff, Program.mem_getConstants_iff, Program.HerbrandBase, Atom.predicate]
-  grind
+#eval Program.hb [Prog|
+parent(xerces, brooke).
+parent(brooke, damocles).
+ancestor(X, Y) :- parent(X, Y).
+ancestor(X, Y) :- parent(X, Z), ancestor(Z, Y).
+]
+
+theorem Program.mem_hb {prog : Program} :
+    ∀ a, a ∈ prog.hb ↔ a.predicate ∈ prog.predicates ∧ ∀ t ∈ a.terms, t ∈ prog.constants := by
+  intro a
+  constructor <;> intro h
+  · constructor
+    · simp [Program.hb] at h
+      obtain ⟨rel, arity, hpreds, tup, hconsts, htup⟩ := h
+      simp [Program.mem_predicates, Atom.predicate] at *
+      simp [Finset.mem_cartesianPower] at hconsts
+      grind
+    · intro t ht
+      simp [Program.hb, Finset.mem_cartesianPower] at h
+      grind
+  · simp [Program.hb]
+    use a.rel, a.terms.length
+    constructor
+    · exact h.left
+    · use a.terms
+      simp [Finset.mem_cartesianPower]
+      exact h.right
 
 -- Herbrand model
 
-inductive Program.HerbrandModel (prog : Program) : Atom → Prop where
-  | step : {r : Rule} → r ∈ prog → (σ : Substitution) → ({a : Atom} → a ∈ r.body → prog.HerbrandModel (a.applySub σ)) → prog.HerbrandModel (r.head.applySub σ)
+inductive Program.HM (prog : Program) : Atom → Prop where
+  | cons : ∀ r ∈ prog, ∀ σ, (∀ a ∈ r.body, prog.HM (a.applySub σ)) → prog.HM (r.head.applySub σ)
+
+def Program.hm (prog : Program) : Set Atom :=
+  {atom | prog.HM atom}
 
 -- Safety
 
@@ -71,63 +269,143 @@ ancestor(X, Y) :- parent(X, Z), ancestor(Z, Y).
 
 -- Finiteness
 
-theorem HerbrandModel_subseteq_HerbrandBase (prog : Program) (safety : prog.IsSafe) (atom : Atom) :
-    prog.HerbrandModel atom → prog.HerbrandBase atom := by
-  intro h
+theorem Program.hm_subset_hb {prog : Program} {safety : prog.IsSafe} :
+    prog.hm ⊆ prog.hb := by
+  intro _ h
   induction h with
-  | step hr σ hbody ih =>
-    rename_i r
+  | cons r hr σ _ ih =>
+    simp [Program.mem_hb]
     constructor
-    · simp [Program.Predicates, Atom.predicate, Atom.applySub]
+    · simp [Program.mem_predicates, Atom.predicate, Atom.applySub]
       grind
     · intro t ht
+      simp [Program.mem_constants]
       constructor
-      · exact isConst_of_mem_applySub ht
+      · suffices r.head.applySub σ |>.isGround by
+          simp [Atom.isGround] at this
+          exact this t ht
+        exact Atom.isGround_of_applySub
       · cases Classical.em (t ∈ r.head.terms) with
         | inl hhead => exact ⟨r, hr, .inl hhead⟩
         | inr hhead =>
-          have ⟨s, hs⟩ : ∃ s, .var s ∈ r.head.terms ∧ .const (σ s) = t := by
-            simp [Atom.applySub, Term.applySub, List.mem_map] at ht
+          have ⟨v, hv⟩ : ∃ s, .var s ∈ r.head.terms ∧ .const (σ s) = t := by
+            simp [Atom.applySub, Term.applySub] at ht
             grind
-          have ⟨a, ha⟩ := (safety r hr) (.var s) hs.left (by simp [Term.isVar])
-          have : t ∈ (a.applySub σ).terms := by
+          have ⟨a, ha⟩ := (safety r hr) (.var v) hv.left (by simp [Term.isVar])
+          have ht' : t ∈ (a.applySub σ).terms := by
             simp [Atom.applySub, Term.applySub]
             grind
-          simp [Program.HerbrandBase, Program.Constants] at ih
+          simp [Program.mem_hb, Program.mem_constants] at ih
           grind
 
 -- Fixpoint semantics
 
-def Subseteq {α : Type} (s₁ s₂ : α → Prop) : Prop :=
-  ∀ e, s₁ e → s₂ e
+def Program.cons (prog : Program) (db : Set Atom) : Set Atom :=
+  {atom | ∃ r ∈ prog, ∃ σ, r.head.applySub σ = atom ∧ ∀ a ∈ r.body, a.applySub σ ∈ db}
 
-infix:50 " ⊆ " => Subseteq
+def Program.lfp (prog : Program) : Set Atom :=
+  {atom | ∀ db, prog.cons db ⊆ db → atom ∈ db}
 
-def Program.ImmediateConsequence (prog : Program) (db : Atom → Prop) (atom : Atom) : Prop :=
-  ∃ r ∈ prog, ∃ σ, r.head.applySub σ = atom ∧ ∀ a ∈ r.body, db (a.applySub σ)
-
-def Program.LeastFixedPoint (prog : Program) (atom : Atom) : Prop :=
-  ∀ db, prog.ImmediateConsequence db ⊆ db → db atom
-
-theorem ImmediateConsequence_monotonic (prog : Program) :
-    ∀ db₁ db₂, db₁ ⊆ db₂ → prog.ImmediateConsequence db₁ ⊆ prog.ImmediateConsequence db₂ := by
+theorem cons_monotonic (prog : Program) :
+    ∀ db₁ db₂, db₁ ⊆ db₂ → prog.cons db₁ ⊆ prog.cons db₂ := by
   intro db₁ db₂ h
-  simp [Subseteq, Program.ImmediateConsequence]
+  simp [Program.cons]
   intro a r hr σ hσ hbody
-  refine ⟨r, hr, σ, hσ, ?_⟩
-  simp [Subseteq] at h
-  grind
+  use r, hr, σ, hσ
+  intro a ha
+  apply h
+  exact hbody a ha
 
-theorem HerbrandModel_iff_LeastFixedPoint (prog : Program) (atom : Atom) :
-    prog.HerbrandModel atom ↔ prog.LeastFixedPoint atom := by
+theorem Program.hm_eq_lfp {prog : Program} :
+    prog.hm = prog.lfp := by
+  ext
   constructor
   · intro h db hdb
     induction h with
-    | step hr σ _ ih =>
+    | cons r hr σ _ ih =>
       apply hdb
-      exact ⟨_, hr, σ, rfl, fun _ => ih⟩
+      exact ⟨r, hr, σ, rfl, ih⟩
   · intro h
     apply h
     intro a ⟨r, hr, σ, hσ, hbody⟩
     rw [← hσ]
-    apply Program.HerbrandModel.step hr _ (fun {a} ha => hbody a ha)
+    apply Program.HM.cons r hr σ hbody
+
+-- Interpreter
+
+abbrev SubstitutionC :=
+  List (Variable × Constant)
+
+def Term.applySubC (sub : SubstitutionC) : Term → Term
+  | .const c => .const c
+  | .var v => .const (sub.lookup v |>.getD "")
+
+def Atom.applySubC (sub : SubstitutionC) (atom : Atom) : Atom :=
+  Atom.mk atom.rel (atom.terms.map (Term.applySubC sub))
+
+def SubstitutionC.toFun (sub : SubstitutionC) : String → String :=
+  fun v => sub.lookup v |>.getD ""
+
+theorem Term.applySubC_eq_applySub_toFun {term : Term} {sub : SubstitutionC} :
+    term.applySubC sub = term.applySub sub.toFun := by
+  simp [Term.applySubC, Term.applySub, SubstitutionC.toFun]
+
+theorem Atom.applySubC_eq_applySub_toFun {atom : Atom} {sub : SubstitutionC} :
+    atom.applySubC sub = atom.applySub sub.toFun := by
+  simp [Atom.applySubC, Atom.applySub]
+  intro t ht
+  exact Term.applySubC_eq_applySub_toFun
+
+def Atom.patternMatch (pattern target : Atom) (sub : SubstitutionC := []) : Option SubstitutionC :=
+  if pattern.predicate = target.predicate then
+    pattern.terms.zip target.terms |>.foldl (fun acc (t₁, t₂) =>
+      match acc with
+      | some sub =>
+        match t₁, t₂ with
+        | .const c₁, .const c₂ => if c₁ = c₂ then sub else none
+        | .var v, .const c =>
+          match sub.lookup v with
+          | some c' => if c = c' then sub else none
+          | none => (v, c) :: sub
+        | _, _ => none
+      | none => none
+    ) (some sub)
+  else
+    none
+
+#eval [Atom| parent(X, Y)].patternMatch [Atom| parent(xerces, brooke)]
+#eval [Atom| parent(X, Y)].patternMatch [Atom| ancestor(xerces, brooke)]
+#eval [Atom| parent(X, Y)].patternMatch [Atom| parent(xerces, brooke, damocles)]
+#eval [Atom| parent(X, X)].patternMatch [Atom| parent(xerces, brooke)]
+#eval [Atom| parent(X, X)].patternMatch [Atom| parent(xerces, xerces)]
+
+def Rule.getSubs (rule : Rule) (db : List Atom) : List SubstitutionC :=
+  rule.body.foldl (fun subs pattern =>
+    subs.flatMap (fun sub =>
+      db.filterMap (fun target =>
+        pattern.patternMatch target sub
+      )
+    )
+  ) [[]]
+
+def Program.step (prog : Program) (db : List Atom) : List Atom :=
+  db.append (prog.flatMap (fun rule =>
+    rule.getSubs db |>.map (fun sub =>
+      Atom.applySubC sub rule.head
+    )
+  ))
+
+def Program.eval (prog : Program) (db : List Atom := []) : Finset Atom :=
+  let db' := prog.step db
+  if db'.toFinset = db.toFinset then db.toFinset else prog.eval db'
+  termination_by
+    (prog.hb \ db.toFinset).card
+  decreasing_by
+    sorry
+
+#eval! Program.eval [Prog|
+parent(xerces, brooke).
+parent(brooke, damocles).
+ancestor(X, Y) :- parent(X, Y).
+ancestor(X, Y) :- parent(X, Z), ancestor(Z, Y).
+]
